Totality improvements and prep for type scheme erasure
type_of is now total in MetaCoq so improve our erasure for this as well.
Also fix some things for upcoming type scheme erasure.

* Make flag_of_type total and improve admitted axiom to actually admit
  something true
* Switch flag_of_type to use our well-founded relation instead of
  MetaCoq's
* Change erase_type to require a proof of isType instead of
  isWfArity_or_Type in preparation for type scheme erasure
* Change erase_type to return TAny for things like stuck fixpoints and
  matches
* Change extended environments to include, for every global declaration,
  whether it includes its dependencies. This is now used to avoid
  printing inductives that are included only because they are matched
  on, and globals that are included purely for deboxing. The old
  ignore_on_print flag on InductiveDecl is now gone as a result.

extraction/theories/Erasure.v
@@ -40,11 +40,13 @@ Import PCUICEnvTyping.
 Import PCUICLookup.
 
 Local Open Scope string_scope.
+Import VectorDef.VectorNotations.
 Import ListNotations.
 Import MonadNotation.
 Set Equations Transparent.
 
 Module P := PCUICAst.
+Module Ex := ExAst.
 
 Import PCUICAst.
 
@@ -107,6 +109,100 @@ Proof.
   eapply isArity_red1; eassumption.
 Qed.
 
+Lemma isType_red Γ t t' :
+  ∥isType Σ Γ t∥ ->
+  ∥red Σ Γ t t'∥ ->
+  ∥isType Σ Γ t'∥.
+Proof.
+  intros [(s & typ)] [r].
+  destruct wfΣ.
+  constructor.
+  exists s.
+  red in typ |- *.
+  eapply subject_reduction; eauto.
+Qed.
+
+Hint Resolve isType_red : erase.
+
+Lemma isType_prod_dom Γ na A B :
+  ∥isType Σ Γ (tProd na A B)∥ ->
+  ∥isType Σ Γ A∥.
+Proof.
+  intros [(s & typ)].
+  destruct wfΣ.
+  apply inversion_Prod in typ as (s' & ? & ? & ? & ?); [|now eauto].
+  constructor.
+  now exists s'.
+Qed.
+
+Hint Resolve isType_prod_dom : erase.
+
+Lemma isType_prod_cod Γ na A B :
+  ∥isType Σ Γ (tProd na A B)∥ ->
+  ∥isType Σ (Γ,, vass na A) B∥.
+Proof.
+  intros [(s & typ)].
+  destruct wfΣ.
+  apply inversion_Prod in typ as (s' & ? & ? & ? & ?); [|now eauto].
+  constructor.
+  now exists x.
+Qed.
+
+Hint Resolve isType_prod_cod : erase.
+
+Lemma isType_isWfArity_or_Type Γ t :
+  ∥isType Σ Γ t∥ ->
+  ∥isWfArity_or_Type Σ Γ t∥.
+Proof.
+  intros [isT].
+  now constructor; right.
+Qed.
+
+Hint Resolve isType_isWfArity_or_Type : erase.
+
+Lemma isWfArity_or_Type_red Γ t t' :
+  ∥isWfArity_or_Type Σ Γ t∥ ->
+  ∥red Σ Γ t t'∥ ->
+  ∥isWfArity_or_Type Σ Γ t'∥.
+Proof.
+  intros.
+  sq.
+  eapply isWfArity_or_Type_red; eauto.
+Qed.
+
+Hint Resolve isWfArity_or_Type_red : erase.
+
+Lemma isWfArity_or_Type_prod_dom Γ na A B :
+  ∥ isWfArity_or_Type Σ Γ (tProd na A B) ∥ ->
+  ∥ isType Σ Γ A ∥.
+Proof.
+  destruct wfΣ as [wfΣu].
+  intros [[ar|isT]].
+  - constructor.
+    apply isWfArity_prod_inv in ar as ((s & ?) & _).
+    now exists s.
+  - pose proof (isType_prod_dom _ _ _ _ (sq isT)).
+    now sq.
+Qed.
+
+Hint Resolve isWfArity_or_Type_prod_dom : erase.
+
+Lemma isWfArity_or_Type_prod_cod Γ na A B :
+  ∥ isWfArity_or_Type Σ Γ (tProd na A B) ∥ ->
+  ∥ isWfArity_or_Type Σ (Γ,, vass na A) B ∥.
+Proof.
+  destruct wfΣ as [wfΣu].
+  intros [[ar|isT]].
+  - constructor; left.
+    apply isWfArity_prod_inv in ar.
+    now destruct ar as ((s & typ) & ar).
+  - pose proof (isType_prod_cod _ _ _ _ (sq isT)).
+    sq.
+    now right.
+Qed.
+
+Hint Resolve isWfArity_or_Type_prod_cod : erase.
+
 Lemma Is_conv_to_Arity_red Γ T T' :
   Is_conv_to_Arity Σ Γ T ->
   ∥ red Σ Γ T T' ∥ ->
@@ -122,164 +218,24 @@ Proof.
   eapply isArity_red; eauto.
 Qed.
 
-Lemma isWfArity_or_Type_prod_cod Γ na A B :
-  ∥ isWfArity_or_Type Σ Γ (tProd na A B) ∥ ->
-  ∥ isWfArity_or_Type Σ (Γ,, vass na A) B ∥.
+Hint Resolve Is_conv_to_Arity_red : erase.
+
+Hint Resolve reduce_term_sound sq existT pair : erase.
+
+Definition is_prod_or_sort (t : term) : bool :=
+  match t with
+  | tProd _ _ _
+  | tSort _ => true
+  | _ => false
+  end.
+
+Lemma not_prod_or_sort_hnf {Γ t wf} :
+  negb (is_prod_or_sort (hnf wfΣ Γ t wf)) ->
+  ~Is_conv_to_Arity Σ Γ t.
 Proof.
-  destruct wfΣ as [wfΣu].
-  intros [[ar|isT]]; constructor.
-  - left.
-    apply isWfArity_prod_inv in ar.
-    now destruct ar as ((s & typ) & ar).
-  - destruct isT as [univ typ].
-    apply inversion_Prod in typ; [|easy].
-    destruct typ as (? & s & ? & ? & ?).
-    right.
-    exists s.
-    easy.
-Qed.
-
-Equations fot_discr (T : term) : Prop :=
-fot_discr (tProd _ _ _) := False;
-fot_discr (tSort _) := False;
-fot_discr _ := True.
-
-Inductive fot_view : term -> Type :=
-| fot_view_prod na A B : fot_view (tProd na A B)
-| fot_view_sort univ : fot_view (tSort univ)
-| fot_view_other t : fot_discr t -> fot_view t.
-
-Equations fot_viewc (t : term) : fot_view t :=
-fot_viewc (tProd na A B) := fot_view_prod na A B;
-fot_viewc (tSort univ) := fot_view_sort univ;
-fot_viewc t := fot_view_other t _.
-
-Lemma watwf {Γ T} (wat : ∥isWfArity_or_Type Σ Γ T∥) : wellformed Σ Γ T.
-Proof. now apply wat_wellformed. Qed.
-
-Axiom hnf_completeness : forall {A}, A.
-Equations(noeqns) flag_of_type (Γ : context) (T : term) (wat : ∥isWfArity_or_Type Σ Γ T∥)
-  : typing_result (type_flag Γ T)
-  by wf ((Γ;T; (watwf wat)) : (∑ Γ t, wellformed Σ Γ t)) term_rel :=
-flag_of_type Γ T wat with inspect (hnf wfΣ Γ T (watwf wat)) :=
-  | exist T is_hnf with fot_viewc T := {
-    | fot_view_prod na A B with flag_of_type (Γ,, vass na A) B _ := {
-      | Checked flag_cod := ret {| is_logical := is_logical flag_cod;
-                                   is_arity := match is_arity flag_cod with
-                                               | left isar => left _
-                                               | right notar => right _
-                                               end;
-                                   is_sort := right _ |};
-      | TypeError t := TypeError t
-      };
-    | fot_view_sort univ := ret {| is_logical := Universe.is_prop univ;
-                                   is_arity := left _;
-                                   is_sort := left _; |};
-    | fot_view_other T discr with infer Σ wfΣ _ Γ T _ := {
-      | exist K princK with reduce_to_sort wfΣ Γ K _ := {
-        | Checked (existT _ univ red_univ) :=
-          ret {| is_logical := Universe.is_prop univ;
-                 is_arity := right _;
-                 is_sort := right _; |};
-        | TypeError t := TypeError t
-        }
-      }
-    }.
-Next Obligation.
-  pose proof (@hnf_sound _ _ wfΣ _ _ (watwf wat)) as [red_hnf].
-  apply isWfArity_or_Type_prod_cod.
-  rewrite is_hnf.
-  destruct wfΣ, wat.
-  sq.
-  eapply isWfArity_or_Type_red; [easy|exact red_hnf|easy].
-Qed.
-Next Obligation.
-  pose proof (@hnf_sound _ _ wfΣ Γ T (watwf wat)) as [sound].
-  sq.
-  exists na, A.
-  rewrite is_hnf.
-  easy.
-Qed.
-Next Obligation.
-  destruct isar as [Bconv [Bred Bar]].
-  exists (tProd na A Bconv).
-  split; [|easy].
-  apply (sq_red_transitivity (tProd na A B)); [rewrite is_hnf; apply hnf_sound|].
-  sq.
-  now apply red_prod_alt.
-Qed.
-Next Obligation.
-  contradiction notar.
-  assert (prod_conv: Is_conv_to_Arity Σ Γ (tProd na A B)).
-  { eapply Is_conv_to_Arity_red with T; [easy|].
-    rewrite is_hnf.
-    apply hnf_sound. }
-  destruct prod_conv as [tm [[redtm] ar]].
-  destruct wfΣ.
-  apply invert_red_prod in redtm; [|easy].
-  destruct redtm as (A' & B' & (-> & redAA') & redBB').
-  exists B'; easy.
-Qed.
-Next Obligation.
-  destruct H as [univ [red_sort]].
-  pose proof (@hnf_sound _ _ wfΣ Γ T (watwf wat)) as [red_prod].
-  rewrite <- is_hnf in red_prod.
-  destruct wfΣ as [wfΣu].
-  pose proof (red_confluence wfΣu red_sort red_prod) as (v' & redv'1 & redv'2).
-  apply invert_red_sort in redv'1.
-  subst.
-  apply invert_red_prod in redv'2 as (? & ? & (? & ?) & ?); easy.
-Qed.
-Next Obligation.
-  exists (tSort univ).
-  split; [|easy].
-  rewrite is_hnf.
-  apply hnf_sound.
-Qed.
-Next Obligation.
-  exists univ.
-  rewrite is_hnf.
-  apply hnf_sound.
-Qed.
-Next Obligation.
-  case wfextΣ.
-  now intros [].
-Qed.
-Next Obligation.
-  destruct wat as [[ar|isT]].
-  - (* We need to show that T is not convertible to an arity under
-       the assumption that hnf of T is neither tProd nor tSort.
-       To do this we will need to use some completeness fact about hnf,
-       which is not proved in MetaCoq yet, so we defer this proof for now. *)
-    exact hnf_completeness.
-  - destruct isT as [[]].
-    now econstructor.
-Qed.
-Next Obligation.
-  destruct princK as [(typK & princK)].
-  apply wat_wellformed; [easy|].
-  destruct wfΣ.
-  sq.
-  eapply validity; [easy|exact typK].
-Qed.
-Next Obligation.
-  (* Same as above: since the head normal form of T is neither a product
-     or sort, it is not convertible to an arity by completeness of hnf. *)
-  exact hnf_completeness.
-Qed.
-Next Obligation.
-  (* Same as above: since the head normal form of T is neither a product
-     or sort, it is not convertible to a sort by completeness of hnf. *)
-  exact hnf_completeness.
-Qed.
-
-Definition redβιζ : RedFlags.t :=
-  {| RedFlags.beta := true;
-     RedFlags.iota := true;
-     RedFlags.zeta := true;
-     RedFlags.delta := false;
-     RedFlags.fix_ := true;
-     RedFlags.cofix_ := true |}.
+  (* We need to use the fact that hnf produces a normal form,
+     but this is not proven in MetaCoq yet, so we admit this for now. *)
+  Admitted.
 
 Inductive term_sub_ctx : context * term -> context * term -> Prop :=
 | sub_prod_dom Γ na A B : term_sub_ctx (Γ, A) (Γ, tProd na A B)
@@ -322,7 +278,7 @@ Proof.
     now rewrite decompose_app_rec_mkApps, atom_decompose_app by easy.
 Qed.
 
-Definition erase_type_rel : Relation_Definitions.relation (∑ Γ t, wellformed Σ Γ t) :=
+Definition erase_rel : Relation_Definitions.relation (∑ Γ t, wellformed Σ Γ t) :=
   fun '(Γs; ts; wfs) '(Γl; tl; wfl) =>
     ∥∑m, red Σ Γl tl m × term_sub_ctx (Γs, ts) (Γl, m)∥.
 
@@ -354,7 +310,7 @@ Proof.
     now apply red_prod_r.
 Qed.
 
-Lemma well_founded_erase_type_rel : well_founded erase_type_rel.
+Lemma well_founded_erase_rel : well_founded erase_rel.
 Proof.
   intros (Γl & l & wfl).
   destruct wfΣ as [wfΣu].
@@ -514,91 +470,156 @@ Proof.
       eapply @normalisation'; eauto.
 Qed.
 
-Instance WellFounded_erase_type_rel : WellFounded erase_type_rel :=
-  Wf.Acc_intro_generator 1000 well_founded_erase_type_rel.
-Opaque WellFounded_erase_type_rel.
+Instance WellFounded_erase_rel : WellFounded erase_rel :=
+  Wf.Acc_intro_generator 1000 well_founded_erase_rel.
+Opaque WellFounded_erase_rel.
 
-Lemma reduce_term_sr {Γ t red wft s} :
-  s = reduce_term red Σ wfΣ Γ t wft ->
-  ∥isWfArity_or_Type Σ Γ t∥ ->
-  ∥isWfArity_or_Type Σ Γ s∥.
-Proof.
-  intros -> [wat].
-  pose proof (reduce_term_sound red Σ wfΣ Γ t wft) as [redt].
+Hint Constructors term_sub_ctx : erase.
+
+Inductive fot_view : term -> Type :=
+| fot_view_prod na A B : fot_view (tProd na A B)
+| fot_view_sort univ : fot_view (tSort univ)
+| fot_view_other t : negb (is_prod_or_sort t) -> fot_view t.
+
+Equations fot_viewc (t : term) : fot_view t :=
+fot_viewc (tProd na A B) := fot_view_prod na A B;
+fot_viewc (tSort univ) := fot_view_sort univ;
+fot_viewc t := fot_view_other t _.
+
+Lemma watwf {Γ T} (wat : ∥isWfArity_or_Type Σ Γ T∥) : wellformed Σ Γ T.
+Proof. now apply wat_wellformed. Qed.
+
+Equations(noeqns) flag_of_type (Γ : context) (T : term) (wat : ∥isWfArity_or_Type Σ Γ T∥)
+  : type_flag Γ T
+  by wf ((Γ;T; (watwf wat)) : (∑ Γ t, wellformed Σ Γ t)) erase_rel :=
+flag_of_type Γ T wat with inspect (hnf wfΣ Γ T (watwf wat)) :=
+  | exist T is_hnf with fot_viewc T := {
+    | fot_view_prod na A B with flag_of_type (Γ,, vass na A) B _ := {
+      | flag_cod := {| is_logical := is_logical flag_cod;
+                       is_arity := match is_arity flag_cod with
+                                   | left isar => left _
+                                   | right notar => right _
+                                   end;
+                       is_sort := right _ |}
+      };
+    | fot_view_sort univ := {| is_logical := Universe.is_prop univ;
+                               is_arity := left _;
+                               is_sort := left _; |};
+    | fot_view_other T discr with infer Σ wfΣ _ Γ T _ := {
+      | exist K princK with inspect (reduce_to_sort wfΣ Γ K _) := {
+        | exist (Checked (existT _ univ red_univ)) eq :=
+          {| is_logical := Universe.is_prop univ;
+             is_arity := right _;
+             is_sort := right _; |};
+        | exist (TypeError t) eq := !
+        }
+    }
+  }.
+
+Ltac reduce_term_sound :=
+  unfold hnf in *;
+  match goal with
+  | [H: ?a = reduce_term ?flags ?Σ ?wfΣ ?Γ ?t ?wft |- _] =>
+    let r := fresh "r" in
+    pose proof (reduce_term_sound flags Σ wfΣ Γ t wft) as [r];
+    rewrite <- H in r
+  end.
+
+Next Obligation. reduce_term_sound; eauto with erase. Qed.
+Next Obligation. reduce_term_sound; eauto with erase. Qed.
+Next Obligation.
+  reduce_term_sound.
+  destruct isar as [Bconv [Bred Bar]].
+  exists (tProd na A Bconv).
+  split; [|easy].
+  apply (sq_red_transitivity (tProd na A B)); [rewrite is_hnf; apply hnf_sound|].
+  sq.
+  now apply red_prod_alt.
+Qed.
+Next Obligation.
+  contradiction notar.
+  assert (prod_conv: Is_conv_to_Arity Σ Γ (tProd na A B)).
+  { eapply Is_conv_to_Arity_red with T; [easy|].
+    rewrite is_hnf.
+    apply hnf_sound. }
+  destruct prod_conv as [tm [[redtm] ar]].
+  destruct wfΣ.
+  apply invert_red_prod in redtm; [|easy].
+  destruct redtm as (A' & B' & (-> & redAA') & redBB').
+  exists B'; easy.
+Qed.
+Next Obligation.
+  destruct H as [univ [red_sort]].
+  pose proof (@hnf_sound _ _ wfΣ Γ T (watwf wat)) as [red_prod].
+  rewrite <- is_hnf in red_prod.
+  destruct wfΣ as [wfΣu].
+  pose proof (red_confluence wfΣu red_sort red_prod) as (v' & redv'1 & redv'2).
+  apply invert_red_sort in redv'1.
+  subst.
+  apply invert_red_prod in redv'2 as (? & ? & (? & ?) & ?); easy.
+Qed.
+Next Obligation.
+  exists (tSort univ).
+  split; [|easy].
+  rewrite is_hnf.
+  apply hnf_sound.
+Qed.
+Next Obligation.
+  exists univ.
+  rewrite is_hnf.
+  apply hnf_sound.
+Qed.
+Next Obligation.
+  case wfextΣ.
+  now intros [].
+Qed.
+Next Obligation.
+  destruct wat as [[ar|isT]].
+  - apply not_prod_or_sort_hnf in discr.
+    now apply nIs_conv_to_Arity_isWfArity_elim in discr.
+  - destruct isT as [[]].
+    now econstructor.
+Qed.
+Next Obligation.
+  destruct princK as [(typK & princK)].
+  apply wat_wellformed; [easy|].
   destruct wfΣ.
   sq.
-  eapply isWfArity_or_Type_red; [easy|exact redt|easy].
+  eapply validity; [easy|exact typK].
+Qed.
+Next Obligation.
+  clear eq.
+  now apply not_prod_or_sort_hnf in discr.
+Qed.
+Next Obligation.
+  clear eq.
+  apply not_prod_or_sort_hnf in discr.
+  contradiction discr.
+  destruct H.
+  exists (tSort x).
+  now split.
+Qed.
+Next Obligation.
+  pose proof (SafeErasureFunction.reduce_to_sort_complete _ (eq_sym eq)).
+  clear eq.
+  apply not_prod_or_sort_hnf in discr.
+  destruct wat as [[|]].
+  - now apply nIs_conv_to_Arity_isWfArity_elim in discr.
+  - destruct i.
+    red in t0.
+    destruct princK as [(typK & princK)].
+    specialize (princK _ t0).
+    eapply invert_cumul_sort_r in princK as (? & ? & ?).
+    eauto.
 Qed.
 
-Lemma isWfArity_or_Type_prod_dom_eq Γ t na A B red wft :
-  ∥ isWfArity_or_Type Σ Γ t ∥ ->
-  tProd na A B = reduce_term red Σ wfΣ Γ t wft ->
-  ∥ isWfArity_or_Type Σ Γ A ∥.
-Proof.
-  intros wat eq.
-  pose proof (reduce_term_sr eq wat) as [wat_prod].
-  clear wat eq.
-  destruct wfΣ as [wfΣu].
-  constructor.
-  right.
-  destruct wat_prod as [ar|isT].
-  - apply isWfArity_prod_inv in ar.
-    destruct ar as ((s & typ) & ar).
-    now econstructor.
-  - destruct isT as [univ typ].
-    apply inversion_Prod in typ; [|easy].
-    destruct typ as (s & ? & ? & ? & ?).
-    exists s.
-    easy.
-Qed.
-
-Lemma isWfArity_or_Type_prod_cod_eq Γ t na A B red wft :
-  ∥ isWfArity_or_Type Σ Γ t ∥ ->
-  tProd na A B = reduce_term red Σ wfΣ Γ t wft ->
-  ∥ isWfArity_or_Type Σ (Γ,, vass na A) B ∥.
-Proof.
-  intros wat eq.
-  pose proof (reduce_term_sr eq wat) as [wat_prod].
-  clear wat eq.
-  destruct wfΣ as [wfΣu].
-  destruct wat_prod as [ar|isT]; constructor.
-  - apply isWfArity_prod_inv in ar.
-    destruct ar as ((s & typ) & ar).
-    now left.
-  - destruct isT as [univ typ].
-    apply inversion_Prod in typ; [|easy].
-    destruct typ as (? & s & ? & ? & ?).
-    right.
-    exists s.
-    easy.
-Qed.
-
-Lemma rec_prod_dom Γ t na A B rf wft :
-  tProd na A B = reduce_term rf Σ wfΣ Γ t wft ->
-  ∥ ∑ r, red Σ Γ t r × term_sub_ctx (Γ, A) (Γ, r) ∥.
-Proof.
-  intros eq.
-  pose proof (reduce_term_sound rf Σ wfΣ Γ t wft) as [red].
-  sq.
-  exists (tProd na A B).
-  split; [rewrite eq; easy|].
-  constructor.
-Qed.
-
-Lemma rec_prod_cod Γ t na A B rf wft :
-  tProd na A B = reduce_term rf Σ wfΣ Γ t wft ->
-  ∥ ∑ r, red Σ Γ t r × term_sub_ctx (Γ,, vass na A, B) (Γ, r) ∥.
-Proof.
-  intros eq.
-  pose proof (reduce_term_sound rf Σ wfΣ Γ t wft) as [red].
-  sq.
-  exists (tProd na A B).
-  split; [rewrite eq; easy|].
-  constructor.
-Qed.
-
-Import VectorDef.VectorNotations.
-Open Scope list.
+Definition redβιζ : RedFlags.t :=
+  {| RedFlags.beta := true;
+     RedFlags.iota := true;
+     RedFlags.zeta := true;
+     RedFlags.delta := false;
+     RedFlags.fix_ := true;
+     RedFlags.cofix_ := true |}.
 
 Equations erase_type_discr (t : term) : Prop := {
   | tRel _ := False;
@@ -660,23 +681,44 @@ Definition wrap_typing_result
   | TypeError te => Err (f te)
   end.
 
+Lemma isTwf {Γ t} (isT: ∥isType Σ Γ t∥) :
+  wellformed Σ Γ t.
+Proof.
+  destruct isT.
+  now apply isType_wellformed.
+Qed.
+
+Definition monad_map_in
+           {T : Type -> Type} {M : Monad T} {A B : Type}
+           (l : list A)
+           (f : forall (a : A), In a l -> T B) : T (list B) :=
+  let fix go (l' : list A) : incl l' l -> T (list B) :=
+      match l' return incl l' l -> T (list B) with
+      | [] => fun _ => ret []
+      | a :: l' =>
+        fun (inc : incl (a :: l') l) =>
+          b <- f a (inc _ (or_introl eq_refl));;
+          tl <- go l' (fun a' a'in => inc _ (or_intror a'in));;
+          ret (b :: tl)
+      end in
+  go l (fun a i => i).
+
 (* Marked noeqns until we need to prove things about it to make its
 definition faster *)
 Equations(noeqns) erase_type
           (Γ : context)
           (erΓ : Vector.t tRel_kind #|Γ|)
           (t : term)
-          (wat : ∥isWfArity_or_Type Σ Γ t∥)
+          (isT : ∥isType Σ Γ t∥)
           (tvars : list name)
   : result (list name × box_type) erase_type_error
-  by wf ((Γ; t; (watwf wat)) : (∑ Γ t, wellformed Σ Γ t)) erase_type_rel :=
-erase_type Γ erΓ t wat tvars with inspect (reduce_term redβιζ Σ wfΣ Γ t (watwf wat)) :=
-  | exist t eq_hnf with (f <- flag_of_type Γ t _;; ret (is_logical f)) := {
-    | TypeError te := Err (TypingError te);
+  by wf ((Γ; t; (isTwf isT)) : (∑ Γ t, wellformed Σ Γ t)) erase_rel :=
+erase_type Γ erΓ t isT tvars with inspect (reduce_term redβιζ Σ wfΣ Γ t (isTwf isT)) :=
+  | exist t eq_hnf with (is_logical (flag_of_type Γ t _)) := {
 
-    | Checked true := ret (tvars, TBox);
+    | true := ret (tvars, TBox);
 
-    | Checked false with erase_type_viewc t := {
+    | false with erase_type_viewc t := {
 
       | et_view_rel i with @Vector.nth_order _ _ erΓ i _ := {
         | RelTypeVar n := ret (tvars, TVar n);
@@ -688,12 +730,12 @@ erase_type Γ erΓ t wat tvars with inspect (reduce_term redβιζ Σ wfΣ Γ t 
 
       | et_view_prod na A B with flag_of_type Γ A _ := {
           (* For logical things, we add a type variable if it's an arity *)
-        | Checked {| is_logical := true |} :=
+        | {| is_logical := true |} :=
           '(tvars, bt) <- erase_type (Γ,, vass na A) (RelOther :: erΓ)%vector B _ tvars;;
           ret (tvars, TArr TBox bt);
 
           (* If the type isn't an arity now, then it's a "normal" type like nat. *)
-        | Checked {| is_arity := right _ |} :=
+        | {| is_arity := right _ |} :=
           '(tvars_dom, dom) <- erase_type Γ erΓ A _ tvars;;
 
           (* If domain added new type vars then it is not in prenex form.
@@ -708,7 +750,7 @@ erase_type Γ erΓ t wat tvars with inspect (reduce_term redβιζ Σ wfΣ Γ t 
           ret (tvars, TArr dom cod);
 
         (* Ok, so it is an arity. If it is a sort then add a type variable. *)
-        | Checked {| is_sort := left _ |} :=
+        | {| is_sort := left _ |} :=
           '(tvars, cod) <- erase_type
                              (Γ,, vass na A) (RelTypeVar (List.length tvars) :: erΓ)%vector
                              B _
@@ -717,9 +759,7 @@ erase_type Γ erΓ t wat tvars with inspect (reduce_term redβιζ Σ wfΣ Γ t 
 
         (* Finally this must be a non-nullary non-logical arity.
            This is not in prenex form. *)
-        | Checked _ := Err NotPrenex;
-
-        | TypeError te := Err (TypingError te)
+        | _ := Err NotPrenex
 
         };
 
@@ -742,8 +782,7 @@ erase_type Γ erΓ t wat tvars with inspect (reduce_term redβιζ Σ wfΣ Γ t 
 
           let erase_arg (a : term) (i : In a decomp_args) : result box_type erase_type_error :=
               let (aT, princaT) := infer Σ wfΣ _ Γ a _ in
-              ft <- wrap_typing_result (flag_of_type Γ aT _) TypingError;;
-              match ft with
+              match flag_of_type Γ aT _ with
               | {| is_logical := true |} => ret TBox
               | {| is_sort := left conv_sort |} =>
                 '(tvars_arg, bt) <- erase_type Γ erΓ a _ tvars;;
@@ -754,19 +793,8 @@ erase_type Γ erΓ t wat tvars with inspect (reduce_term redβιζ Σ wfΣ Γ t 
               | _ => ret TAny (* Arity or value *)
               end in
 
-          let fix erase_args
-                  (args : list term) (inc : incl args decomp_args)
-                  (r : box_type) : result (list name * box_type) erase_type_error :=
-              match args return incl args decomp_args ->
-                                result (list name * box_type) erase_type_error with
-              | [] => fun _ => ret (tvars, r)
-              | a :: args =>
-                fun inc =>
-                  abt <- erase_arg a _;;
-                  erase_args args _ (TApp r abt)
-              end inc in
-
-          erase_args decomp_args _ hdbt
+          args <- monad_map_in decomp_args erase_arg;;
+          ret (tvars, mkTApps hdbt args)
 
         };
 
@@ -774,62 +802,57 @@ erase_type Γ erΓ t wat tvars with inspect (reduce_term redβιζ Σ wfΣ Γ t 
 
       | et_view_ind ind _ := ret (tvars, TInd ind);
 
-      | et_view_other t _ := Err (GeneralError ("Unsupported type " ++ string_of_term t))
+      | et_view_other t _ := ret (tvars, TAny)
 
       }
     }.
-Next Obligation. now eapply reduce_term_sr. Qed.
+Solve All Obligations with
+    Tactics.program_simplify;
+    CoreTactics.equations_simpl;
+    try reduce_term_sound;
+    eauto with erase.
 Next Obligation.
-  pose proof (reduce_term_sr eq_hnf wat) as [wat_rel].
-  destruct wfΣ as [wfΣu].
-  destruct wat_rel as [isar|(univ & typ)].
-  - now destruct isar as (? & ? & ? & ?).
-  - apply inversion_Rel in typ; [|easy].
-    apply nth_error_Some.
-    destruct typ as (? & _ & ? & _).
-    congruence.
+  reduce_term_sound.
+  assert (∥isType Σ Γ (tRel i)∥) as [(s & typ)] by eauto with erase.
+  red in typ.
+  clear eq_hnf.
+  destruct wfΣ.
+  eapply subject_reduction in typ; eauto.
+  apply inversion_Rel in typ as (? & _ & ? & _); [|easy].
+  now apply nth_error_Some.
 Qed.
-Next Obligation. now eapply isWfArity_or_Type_prod_dom_eq. Qed.
-Next Obligation. now eapply isWfArity_or_Type_prod_cod_eq. Qed.
-Next Obligation. now eapply rec_prod_cod. Qed.
-Next Obligation. now eapply isWfArity_or_Type_prod_cod_eq. Qed.
-Next Obligation. now eapply rec_prod_cod. Qed.
-Next Obligation. now eapply isWfArity_or_Type_prod_dom_eq. Qed.
-Next Obligation. now eapply rec_prod_dom. Qed.
-Next Obligation. now eapply isWfArity_or_Type_prod_cod_eq. Qed.
-Next Obligation. now eapply rec_prod_cod. Qed.
 Next Obligation.
-  pose proof (reduce_term_sr eq_hnf wat) as [[isar|(univ & typ)]].
-  - now destruct isar as (? & ? & ? & ?).
-  - unfold PCUICTypingDef.typing in typ.
-    replace (tApp orig_hd orig_arg) with (mkApps (tRel i) decomp_args) in typ; cycle 1.
-    { symmetry. apply decompose_app_inv.
-      now rewrite <- eq_decomp. }
-    destruct wfΣ as [wfΣu].
-    apply inversion_mkApps in typ; [|easy].
-    destruct typ as (rel_type & rel_typed & spine).
-    apply inversion_Rel in rel_typed; [|easy].
-    apply nth_error_Some.
-    destruct rel_typed as (? & _ & ? & _).
-    congruence.
+  reduce_term_sound; clear eq_hnf.
+  destruct isT as [(? & typ)].
+  destruct wfΣ.
+  eapply subject_reduction in typ; eauto.
+  replace (tApp orig_hd orig_arg) with (mkApps (tRel i) decomp_args) in typ; cycle 1.
+  { symmetry. apply decompose_app_inv.
+    now rewrite <- eq_decomp. }
+  apply inversion_mkApps in typ; [|easy].
+  destruct typ as (rel_type & rel_typed & spine).
+  apply inversion_Rel in rel_typed; [|easy].
+  apply nth_error_Some.
+  destruct rel_typed as (? & _ & ? & _).
+  congruence.
 Qed.
 Next Obligation. now case wfextΣ; intros [[]]. Qed.
 Next Obligation.
-  pose proof (reduce_term_sr eq_hnf wat) as [[isar|(univ & typ)]].
-  - now destruct isar as (? & ? & ? & ?).
-  - unfold PCUICTypingDef.typing in typ.
-    replace (tApp orig_hd orig_arg) with (mkApps hd decomp_args) in typ; cycle 1.
-    { symmetry. apply decompose_app_inv.
-      now rewrite <- eq_decomp. }
-    destruct wfΣ as [wfΣu].
-    apply inversion_mkApps in typ; [|easy].
-    destruct typ as (? & ? & spine).
-    clear -spine i.
-    induction spine; [easy|].
-    destruct i.
-    + subst a.
-      econstructor; easy.
-    + easy.
+  reduce_term_sound; clear eq_hnf.
+  destruct isT as [(? & typ)].
+  destruct wfΣ.
+  eapply subject_reduction in typ; eauto.
+  replace (tApp orig_hd orig_arg) with (mkApps hd decomp_args) in typ; cycle 1.
+  { symmetry. apply decompose_app_inv.
+    now rewrite <- eq_decomp. }
+  apply inversion_mkApps in typ; [|easy].
+  destruct typ as (? & ? & spine).
+  clear -spine i.
+  induction spine; [easy|].
+  destruct i.
+  + subst a.
+    econstructor; easy.
+  + easy.
 Qed.
 Next Obligation.
   destruct princaT as [(typ & princaT)].
@@ -842,24 +865,17 @@ Next Obligation.
   destruct conv_sort as (univ & reduniv).
   destruct wfΣ as [wfΣu].
   sq.
-  right.
   exists univ.
   eapply type_reduction; [easy|exact typ|easy].
 Qed.
 Next Obligation.
-  pose proof (reduce_term_sound redβιζ Σ wfΣ Γ t (watwf wat)).
+  reduce_term_sound; clear eq_hnf.
   sq.
   exists (tApp orig_hd orig_arg).
-  split; [rewrite eq_hnf; easy|].
+  split; [easy|].
   constructor.
   rewrite <- eq_decomp.
   easy.
-Qed.
-Next Obligation.
-  now specialize (inc a (or_introl eq_refl)).
-Qed.
-Next Obligation.
-  now specialize (inc a0 (or_intror H)).
 Qed.
 
 Inductive erase_constant_decl_error :=
@@ -873,72 +889,67 @@ Definition string_of_erase_constant_decl_error (err : erase_constant_decl_error)
   end.
 
 Import ExAst.
-Program Definition erase_constant_decl
+Equations? (noeqns) erase_constant_decl
           (cst : P.constant_body)
           (wt : ∥on_constant_decl (lift_typing typing) Σ cst∥)
   : result (constant_body + (list name × box_type)) erase_constant_decl_error :=
-  flg <- wrap_typing_result (flag_of_type [] (P.cst_type cst) _) EraseBodyError ;;
-  match is_sort flg with
-  | left ics => (* erase as a type alias  *)
-    match P.cst_body cst with
-    | Some body =>
-      ety <- map_error EraseTypeError (erase_type [] []%vector body _ []);;
-      ret (inr ety)
-    | None =>
-      Err (EraseBodyError (Msg "Type alias without a body"))
-    end
-  | right _ => (* proceed as usual *)
-    et <- map_error EraseTypeError (erase_type [] []%vector (P.cst_type cst) _ []);;
-    let eb :=
-        match P.cst_body cst with
-         | Some body => Some (SafeErasureFunction.erase Σ wfextΣ [] body _)
-         | None => None
-        end in
-    ret (inl {| cst_type := et; cst_body := eb |})
-  end.
-Next Obligation.
-  sq.
-  unfold on_constant_decl in wt.
-  destruct (P.cst_body cst).
-  - cbn in wt.
-    eapply validity_term; [easy|exact wt].
-  - cbn in wt.
-    destruct wt as (s & ?).
-    right.
-    now exists s.
-Qed.
-Next Obligation.
-  destruct ics as [u Hred].
-  destruct Hred as [Hred].
-  sq.
-  unfold on_constant_decl in wt.
-  destruct (P.cst_body cst).
-  - cbn in wt.
-    inversion Heq_anonymous;subst.
-    right. exists u.
-    eapply type_reduction;eauto.
-  - cbn in wt.
-    destruct wt as (s & ?).
-    right.
-    now exists s.
-Qed.
-Next Obligation.
-  sq.
-  unfold on_constant_decl in wt.
-  destruct (P.cst_body cst).
-  - cbn in wt.
-    eapply validity_term; [easy|exact wt].
-  - cbn in wt.
-    destruct wt as (s & ?).
-    right.
-    now exists s.
-Qed.
-Next Obligation.
-  destruct wt as [wt].
-  unfold on_constant_decl in wt.
-  rewrite <- Heq_anonymous in wt.
-  cbn in *.
-  now eapply iswelltyped.
+erase_constant_decl cst wt with flag_of_type [] (P.cst_type cst) _ := {
+  | {| is_arity := left isar; is_sort := left issort |} with inspect (P.cst_body cst) := {
+    | exist (Some body) body_eq with erase_type [] []%vector body _ [] := {
+      | Err err => Err (EraseTypeError err);
+      | Ok ety => Ok (inr ety)
+      };
+    | exist None _ => Err (EraseBodyError (Msg "Type alias without a body"))
+    };
+  | {| is_arity := left isar; is_sort := right notsort |} =>
+    Err (EraseBodyError (Msg "Cannot handle type schemes yet"));
+  | {| is_arity := right notar |} with erase_type [] []%vector (P.cst_type cst) _ [] := {
+    | Err err => Err (EraseTypeError err);
+    | Ok ety with inspect (P.cst_body cst) := {
+      | exist (Some body) body_eq =>
+        Ok (inl {| cst_type := ety;
+                   cst_body := Some (SafeErasureFunction.erase Σ wfextΣ [] body _) |});
+      | exist None _ => Ok (inl {| cst_type := ety; cst_body := None |})
+      }
+    }
+  }.
+Proof.
+  - sq.
+    unfold on_constant_decl in wt.
+    destruct (P.cst_body cst).
+    + cbn in wt.
+      eapply validity_term; [easy|exact wt].
+    + cbn in wt.
+      destruct wt as (s & ?).
+      right.
+      now exists s.
+  - destruct cst; cbn in *.
+    subst cst_body.
+    cbn in *.
+    destruct issort as (s & [r]).
+    sq.
+    exists s.
+    red.
+    eapply type_reduction; eauto.
+  - destruct wfΣ.
+    destruct wt as [wt].
+    unfold on_constant_decl in wt.
+    destruct (P.cst_body cst).
+    + cbn in wt.
+      eapply validity_term in wt; [|now eauto].
+      destruct wt.
+      * now apply nIs_conv_to_Arity_isWfArity_elim in notar.
+      * now constructor.
+    + cbn in wt.
+      destruct wt as (s & ?).
+      constructor.
+      now exists s.
+  - destruct wt as [wt].
+    unfold on_constant_decl in wt.
+    rewrite <- body_eq in wt.
+    cbn in *.
+    econstructor.
+    eassumption.
 Qed.
 
 Import P.
@@ -949,25 +960,24 @@ Definition fot_to_oib_tvar (na : name) {Γ t} (f : type_flag Γ t) : oib_type_va
      tvar_is_arity := if is_arity f then true else false;
      tvar_is_sort := if is_sort f then true else false; |}.
 
-Equations erase_ind_arity
+Equations? (noeqns) erase_ind_arity
           (Γ : context)
           (t : term)
           (wat : ∥isWfArity_or_Type Σ Γ t∥)
   : typing_result (list oib_type_var)
-  by wf ((Γ; t; watwf wat) : (∑ Γ t, wellformed Σ Γ t)) erase_type_rel :=
+  by wf ((Γ; t; watwf wat) : (∑ Γ t, wellformed Σ Γ t)) erase_rel :=
 erase_ind_arity Γ t wat with inspect (hnf wfΣ Γ t (watwf wat)) := {
   | exist (tProd na A B) hnf_eq with flag_of_type Γ A _ := {
-    | TypeError te := TypeError te;
-    | Checked f with erase_ind_arity (Γ,, vass na A) B _ := {
+    | f with erase_ind_arity (Γ,, vass na A) B _ := {
       | TypeError te := TypeError te;
       | Checked tvars := ret (fot_to_oib_tvar na f :: tvars)
       }
     };
   | exist _ _ := ret []
   }.
-Next Obligation. now eapply isWfArity_or_Type_prod_dom_eq. Qed.
-Next Obligation. now eapply isWfArity_or_Type_prod_cod_eq. Qed.
-Next Obligation. now eapply rec_prod_cod. Qed.
+Proof.
+  all: reduce_term_sound; eauto with erase.
+Qed.
 
 Definition arities_contexts
          (mind : kername)
@@ -1031,21 +1041,6 @@ Definition string_of_erase_ind_body_error (e : erase_ind_body_error) : string :=
   | CtorUnmappedTypeVariables ctor => "Ctor " ++ ctor ++ " has unmapped type variables"
   end.
 
-Definition monad_map_in
-           {T : Type -> Type} {M : Monad T} {A B : Type}
-           (l : list A)
-           (f : forall (a : A), In a l -> T B) : T (list B) :=
-  let fix go (l' : list A) : incl l' l -> T (list B) :=
-      match l' return incl l' l -> T (list B) with
-      | [] => fun _ => ret []
-      | a :: l' =>
-        fun (inc : incl (a :: l') l) =>
-          b <- f a (inc _ (or_introl eq_refl));;
-          tl <- go l' (fun a' a'in => inc _ (or_intror a'in));;
-          ret (b :: tl)
-      end in
-  go l (fun a i => i).
-
 Program Definition erase_ind_body
         (mind : kername)
         (mib : P.mutual_inductive_body)
@@ -1096,7 +1091,6 @@ Next Obligation.
   induction on_ctors; [easy|].
   destruct is_in as [->|later]; [|easy].
   constructor.
-  right.
   destruct (on_ctype r) as (s & typ).
   rewrite <- (arities_contexts_1 mind) in typ.
   rewrite <- Heq_anonymous in typ.
@@ -1132,21 +1126,18 @@ Next Obligation.
   constructor.
   exists i.
   specialize (onInductives _ _ _ _ wt).
+
+  change i with (0 + i).
+  generalize 0 as n.
   revert i nth_some.
 
-  enough (H: forall n i,
-             nth_error (P.ind_bodies mib) i = Some oib ->
-             Alli (on_ind_body (lift_typing typing) Σ kn mib) n (P.ind_bodies mib) ->
-             on_ind_body (lift_typing typing) Σ kn mib (n + i) oib).
-  { apply (H 0). }
-
-  induction (P.ind_bodies mib) as [|? oibs IH]; intros n i nth_some inds_wt.
+  induction (P.ind_bodies mib) as [|? oibs IH]; intros i nth_some n inds_wt.
   - now rewrite nth_error_nil in nth_some.
   - inversion inds_wt; subst; clear inds_wt.
     destruct i; cbn in *.
     + replace a with oib in * by congruence.
       now rewrite Nat.add_0_r.
-    + specialize (IH (S n)).
+    + specialize (IH _ nth_some (S n)).
       now rewrite Nat.add_succ_r.
 Qed.
 
@@ -1188,7 +1179,7 @@ Program Definition erase_global_decl
   | P.InductiveDecl mib =>
     ind <- map_error (ErrInductive Σext kn)
                      (erase_ind Σext _ kn mib _);;
-    ret (InductiveDecl false ind)
+    ret (InductiveDecl ind)
   end.
 
 Definition add_seen (n : kername) (seen : list kername) : list kername :=
@@ -1237,7 +1228,7 @@ Definition decl_deps (seen : list kername) (decl : global_decl) : list kername :
         | None => seen
         end in
     box_type_deps seen (cst_type body).2
-  | InductiveDecl _ mib =>
+  | InductiveDecl mib =>
     let one_inductive_body_deps seen oib :=
         let seen := fold_left box_type_deps
                               (flat_map snd (ind_ctors oib))
@@ -1256,60 +1247,36 @@ Definition is_inductive_decl (d : P.global_decl) : bool :=
 Definition contains (kn : kername) :=
   List.existsb (eq_kername kn).
 
-(* Erase the global declarations by the specified names and
-   their non-erased dependencies recursively. Ignore dependencies for which [ignore] returnes [true] *)
+(* Erase the global declarations by the specified names and their
+   non-erased dependencies recursively. Ignore dependencies for which
+   [ignore_deps] returnes [true] *)
 Program Fixpoint erase_global_decls_deps_recursive
         (Σ : P.global_env)
         (wfΣ : ∥wf Σ∥)
         (include : list kername)
-        (ignore : kername -> bool)
+        (ignore_deps : kername -> bool)
   : result global_env erase_global_decl_error :=
   match Σ with
   | [] => ret []
   | (kn, decl) :: Σ =>
     let Σext := (Σ, universes_decl_of_decl decl) in
     if contains kn include then
-      if ignore kn then
-      (* NOTE: if we ignore an inductive declaration, we still add
-      it to have enough info for printing [match] and inductives that
-      depend on it. But we ignore its dependencies and ignore the
-      declaration itself on printing.
-      This is a bit of a hack, we should probably not erase (all) ignored
-      types as they may fail to erase. *)
-        decl <-
-        match decl with
-        | P.InductiveDecl mib =>
-          ind <- map_error (ErrInductive Σext kn)
-                           (erase_ind Σext _ kn mib _);;
-        ret (kn, InductiveDecl true ind)
-        | P.ConstantDecl cb =>
-          ety <- map_error ((ErrConstant Σext kn) ∘ EraseTypeError)
-                          (erase_type Σext _ [] (Vector.nil _) cb.(P.cst_type) _ []);;
-          let cb' := {| cst_type := ety; cst_body := None |} in
-          ret (kn, ConstantDecl cb')
-        end;;
-        Σer <- erase_global_decls_deps_recursive Σ _ include ignore;;
-        ret (decl :: Σer)%list
-      else
-        decl <- erase_global_decl Σext _ kn decl _;;
-        Σer <- erase_global_decls_deps_recursive Σ _ (decl_deps include decl) ignore;;
-        ret ((kn, decl) :: Σer)
+      (* We still erase ignored inductives and constants for two reasons:
+         1. For inductives, we want to allow pattern matches on them and we need
+         information about them to print names.
+         2. For constants, we use their type to do deboxing.
+         This is a little hacky as we might fail to erase these and then fail erasure.
+         On the other hand, it is unlikely that something remapped has a higher-kinded type
+         as we wouldn't be able to remap it to something sane, so this is probably ok. *)
+      decl <- erase_global_decl Σext _ kn decl _;;
+      let with_deps := negb (ignore_deps kn) in
+      let new_deps := if with_deps then decl_deps include decl else include in
+      Σer <- erase_global_decls_deps_recursive Σ _ new_deps ignore_deps;;
+      ret ((kn, with_deps, decl) :: Σer)
     else
-      erase_global_decls_deps_recursive Σ _ include ignore
+      erase_global_decls_deps_recursive Σ _ include ignore_deps
   end.
 Solve Obligations with try now cbn;intros;subst; sq; inversion wfΣ.
-Next Obligation.
-  sq.
-  inversion wfΣ;subst;clear wfΣ;cbn in *.
-  unfold on_constant_decl in *.
-  destruct (P.cst_body cb).
-  - cbn in *.
-    eapply validity_term; [easy|eassumption].
-  - cbn in *.
-    destruct X0 as (s & ?).
-    right.
-    now exists s.
-Qed.
 
 End EraseEnv.
 
